More generic and useful queue spec.

progs/queue_ex.c
@@ -9,10 +9,12 @@ int results[3][3];
 
 void *f(void *arg){
   int t = *(int *)arg;
+  queue_t *q1 = q0;
 
   for(int i = 0; i < 3; i++){
-    int *d = (int *)q_remove(q0);
+    int *d = (int *)q_remove(q1);
     int v = *d;
+    free(d);
     results[t][i] = v;
   }
   
@@ -23,7 +25,8 @@ void *f(void *arg){
 
 int main(void){
   int tid[3] = {0, 1, 2};
-
+  queue_t *q1 = q0;
+  
   q0 = q_new();
 
   for(int i = 0; i < 3; i++){
@@ -37,7 +40,7 @@ int main(void){
   for(int i = 0; i < 9; i++){
     int *d = (int *)malloc(sizeof(int));
     *d = i;
-    q_add(q0, d);
+    q_add(q1, d);
   }
 
   for(int i = 0; i < 3; i++){
@@ -47,12 +50,11 @@ int main(void){
     free(l);
   }
 
-  queue_t *q1 = q0;
   q_del(q1);
 
-  for(int i = 0; i < 3; i++)
+  /*  for(int i = 0; i < 3; i++)
     for(int j = 0; j < 3; j++)
-      printf("%d ", results[i][j]);
+    printf("%d ", results[i][j]);*/
       
   //results should merge to input
 }
