progs/queue_ex.v
@@ -49,11 +49,10 @@ Definition ___i64_udiv : ident := 33%positive.
 Definition ___i64_umod : ident := 35%positive.
 Definition ___i64_utod : ident := 29%positive.
 Definition ___i64_utof : ident := 31%positive.
-Definition ___stringlit_1 : ident := 109%positive.
 Definition _a : ident := 1%positive.
 Definition _acquire : ident := 66%positive.
 Definition _addc : ident := 7%positive.
-Definition _arg : ident := 99%positive.
+Definition _arg : ident := 98%positive.
 Definition _buf : ident := 3%positive.
 Definition _c : ident := 78%positive.
 Definition _c__1 : ident := 86%positive.
@@ -63,14 +62,12 @@ Definition _f : ident := 101%positive.
 Definition _free : ident := 62%positive.
 Definition _freecond : ident := 69%positive.
 Definition _freelock : ident := 65%positive.
-Definition _freelock2 : ident := 93%positive.
+Definition _freelock2 : ident := 92%positive.
 Definition _h : ident := 88%positive.
 Definition _head : ident := 5%positive.
 Definition _i : ident := 77%positive.
 Definition _i__1 : ident := 103%positive.
 Definition _i__2 : ident := 104%positive.
-Definition _i__3 : ident := 107%positive.
-Definition _j : ident := 108%positive.
 Definition _l : ident := 79%positive.
 Definition _l__1 : ident := 105%positive.
 Definition _len : ident := 84%positive.
@@ -84,10 +81,9 @@ Definition _malloc : ident := 63%positive.
 Definition _n : ident := 72%positive.
 Definition _newq : ident := 75%positive.
 Definition _p : ident := 73%positive.
-Definition _printf : ident := 92%positive.
 Definition _q : ident := 76%positive.
-Definition _q0 : ident := 96%positive.
-Definition _q1 : ident := 106%positive.
+Definition _q0 : ident := 95%positive.
+Definition _q1 : ident := 99%positive.
 Definition _q_add : ident := 87%positive.
 Definition _q_del : ident := 82%positive.
 Definition _q_new : ident := 80%positive.
@@ -97,31 +93,23 @@ Definition _queue : ident := 9%positive.
 Definition _queue_t : ident := 12%positive.
 Definition _r : ident := 83%positive.
 Definition _release : ident := 67%positive.
-Definition _release2 : ident := 94%positive.
+Definition _release2 : ident := 93%positive.
 Definition _remc : ident := 8%positive.
-Definition _results : ident := 98%positive.
+Definition _results : ident := 97%positive.
 Definition _signalcond : ident := 71%positive.
-Definition _spawn : ident := 95%positive.
+Definition _spawn : ident := 94%positive.
 Definition _surely_malloc : ident := 74%positive.
 Definition _t : ident := 85%positive.
 Definition _tail : ident := 6%positive.
 Definition _tgt : ident := 81%positive.
-Definition _thread_locks : ident := 97%positive.
+Definition _thread_locks : ident := 96%positive.
 Definition _tid : ident := 102%positive.
 Definition _v : ident := 100%positive.
 Definition _waitcond : ident := 70%positive.
-Definition _t'1 : ident := 110%positive.
-Definition _t'2 : ident := 111%positive.
-Definition _t'3 : ident := 112%positive.
-Definition _t'4 : ident := 113%positive.
-
-Definition v___stringlit_1 := {|
-  gvar_info := (tarray tschar 4);
-  gvar_init := (Init_int8 (Int.repr 37) :: Init_int8 (Int.repr 100) ::
-                Init_int8 (Int.repr 32) :: Init_int8 (Int.repr 0) :: nil);
-  gvar_readonly := true;
-  gvar_volatile := false
-|}.
+Definition _t'1 : ident := 106%positive.
+Definition _t'2 : ident := 107%positive.
+Definition _t'3 : ident := 108%positive.
+Definition _t'4 : ident := 109%positive.
 
 Definition f_surely_malloc := {|
   fn_return := (tptr tvoid);
@@ -689,55 +677,64 @@ Definition f_f := {|
   fn_callconv := cc_default;
   fn_params := ((_arg, (tptr tvoid)) :: nil);
   fn_vars := nil;
-  fn_temps := ((_t, tint) :: (_i, tint) :: (_d, (tptr tint)) :: (_v, tint) ::
+  fn_temps := ((_t, tint) :: (_q1, (tptr (Tstruct _queue_t noattr))) ::
+               (_i, tint) :: (_d, (tptr tint)) :: (_v, tint) ::
                (_l, (tptr (Tstruct _lock_t noattr))) ::
                (_t'1, (tptr tvoid)) :: nil);
   fn_body :=
 (Ssequence
   (Sset _t (Ederef (Ecast (Etempvar _arg (tptr tvoid)) (tptr tint)) tint))
   (Ssequence
+    (Sset _q1 (Evar _q0 (tptr (Tstruct _queue_t noattr))))
     (Ssequence
-      (Sset _i (Econst_int (Int.repr 0) tint))
-      (Sloop
-        (Ssequence
-          (Sifthenelse (Ebinop Olt (Etempvar _i tint)
-                         (Econst_int (Int.repr 3) tint) tint)
-            Sskip
-            Sbreak)
-          (Ssequence
-            (Ssequence
-              (Scall (Some _t'1)
-                (Evar _q_remove (Tfunction
-                                  (Tcons (tptr (Tstruct _queue_t noattr))
-                                    Tnil) (tptr tvoid) cc_default))
-                ((Evar _q0 (tptr (Tstruct _queue_t noattr))) :: nil))
-              (Sset _d (Ecast (Etempvar _t'1 (tptr tvoid)) (tptr tint))))
-            (Ssequence
-              (Sset _v (Ederef (Etempvar _d (tptr tint)) tint))
-              (Sassign
-                (Ederef
-                  (Ebinop Oadd
-                    (Ederef
-                      (Ebinop Oadd (Evar _results (tarray (tarray tint 3) 3))
-                        (Etempvar _t tint) (tptr (tarray tint 3)))
-                      (tarray tint 3)) (Etempvar _i tint) (tptr tint)) tint)
-                (Etempvar _v tint)))))
-        (Sset _i
-          (Ebinop Oadd (Etempvar _i tint) (Econst_int (Int.repr 1) tint)
-            tint))))
-    (Ssequence
-      (Sset _l
-        (Ederef
-          (Ebinop Oadd
-            (Evar _thread_locks (tarray (tptr (Tstruct _lock_t noattr)) 3))
-            (Etempvar _t tint) (tptr (tptr (Tstruct _lock_t noattr))))
-          (tptr (Tstruct _lock_t noattr))))
       (Ssequence
-        (Scall None
-          (Evar _release2 (Tfunction (Tcons (tptr tvoid) Tnil) tvoid
-                            cc_default))
-          ((Etempvar _l (tptr (Tstruct _lock_t noattr))) :: nil))
-        (Sreturn (Some (Econst_int (Int.repr 0) tint)))))))
+        (Sset _i (Econst_int (Int.repr 0) tint))
+        (Sloop
+          (Ssequence
+            (Sifthenelse (Ebinop Olt (Etempvar _i tint)
+                           (Econst_int (Int.repr 3) tint) tint)
+              Sskip
+              Sbreak)
+            (Ssequence
+              (Ssequence
+                (Scall (Some _t'1)
+                  (Evar _q_remove (Tfunction
+                                    (Tcons (tptr (Tstruct _queue_t noattr))
+                                      Tnil) (tptr tvoid) cc_default))
+                  ((Etempvar _q1 (tptr (Tstruct _queue_t noattr))) :: nil))
+                (Sset _d (Ecast (Etempvar _t'1 (tptr tvoid)) (tptr tint))))
+              (Ssequence
+                (Sset _v (Ederef (Etempvar _d (tptr tint)) tint))
+                (Ssequence
+                  (Scall None
+                    (Evar _free (Tfunction (Tcons (tptr tvoid) Tnil) tvoid
+                                  cc_default))
+                    ((Etempvar _d (tptr tint)) :: nil))
+                  (Sassign
+                    (Ederef
+                      (Ebinop Oadd
+                        (Ederef
+                          (Ebinop Oadd
+                            (Evar _results (tarray (tarray tint 3) 3))
+                            (Etempvar _t tint) (tptr (tarray tint 3)))
+                          (tarray tint 3)) (Etempvar _i tint) (tptr tint))
+                      tint) (Etempvar _v tint))))))
+          (Sset _i
+            (Ebinop Oadd (Etempvar _i tint) (Econst_int (Int.repr 1) tint)
+              tint))))
+      (Ssequence
+        (Sset _l
+          (Ederef
+            (Ebinop Oadd
+              (Evar _thread_locks (tarray (tptr (Tstruct _lock_t noattr)) 3))
+              (Etempvar _t tint) (tptr (tptr (Tstruct _lock_t noattr))))
+            (tptr (Tstruct _lock_t noattr))))
+        (Ssequence
+          (Scall None
+            (Evar _release2 (Tfunction (Tcons (tptr tvoid) Tnil) tvoid
+                              cc_default))
+            ((Etempvar _l (tptr (Tstruct _lock_t noattr))) :: nil))
+          (Sreturn (Some (Econst_int (Int.repr 0) tint))))))))
 |}.
 
 Definition f_main := {|
@@ -745,11 +742,11 @@ Definition f_main := {|
   fn_callconv := cc_default;
   fn_params := nil;
   fn_vars := ((_tid, (tarray tint 3)) :: nil);
-  fn_temps := ((_i, tint) :: (_l, (tptr (Tstruct _lock_t noattr))) ::
-               (_t, (tptr tvoid)) :: (_i__1, tint) :: (_d, (tptr tint)) ::
-               (_i__2, tint) :: (_l__1, (tptr (Tstruct _lock_t noattr))) ::
-               (_q1, (tptr (Tstruct _queue_t noattr))) :: (_i__3, tint) ::
-               (_j, tint) :: (_t'3, (tptr tvoid)) :: (_t'2, (tptr tvoid)) ::
+  fn_temps := ((_q1, (tptr (Tstruct _queue_t noattr))) :: (_i, tint) ::
+               (_l, (tptr (Tstruct _lock_t noattr))) :: (_t, (tptr tvoid)) ::
+               (_i__1, tint) :: (_d, (tptr tint)) :: (_i__2, tint) ::
+               (_l__1, (tptr (Tstruct _lock_t noattr))) ::
+               (_t'3, (tptr tvoid)) :: (_t'2, (tptr tvoid)) ::
                (_t'1, (tptr (Tstruct _queue_t noattr))) :: nil);
   fn_body :=
 (Ssequence
@@ -772,193 +769,153 @@ Definition f_main := {|
               (Econst_int (Int.repr 2) tint) (tptr tint)) tint)
           (Econst_int (Int.repr 2) tint))
         (Ssequence
-          (Ssequence
-            (Scall (Some _t'1)
-              (Evar _q_new (Tfunction Tnil (tptr (Tstruct _queue_t noattr))
-                             cc_default)) nil)
-            (Sassign (Evar _q0 (tptr (Tstruct _queue_t noattr)))
-              (Etempvar _t'1 (tptr (Tstruct _queue_t noattr)))))
+          (Sset _q1 (Evar _q0 (tptr (Tstruct _queue_t noattr))))
           (Ssequence
             (Ssequence
-              (Sset _i (Econst_int (Int.repr 0) tint))
-              (Sloop
-                (Ssequence
-                  (Sifthenelse (Ebinop Olt (Etempvar _i tint)
-                                 (Econst_int (Int.repr 3) tint) tint)
-                    Sskip
-                    Sbreak)
-                  (Ssequence
-                    (Ssequence
-                      (Scall (Some _t'2)
-                        (Evar _malloc (Tfunction (Tcons tuint Tnil)
-                                        (tptr tvoid) cc_default))
-                        ((Esizeof (Tstruct _lock_t noattr) tuint) :: nil))
-                      (Sset _l
-                        (Ecast (Etempvar _t'2 (tptr tvoid))
-                          (tptr (Tstruct _lock_t noattr)))))
-                    (Ssequence
-                      (Sassign
-                        (Ederef
-                          (Ebinop Oadd
-                            (Evar _thread_locks (tarray (tptr (Tstruct _lock_t noattr)) 3))
-                            (Etempvar _i tint)
-                            (tptr (tptr (Tstruct _lock_t noattr))))
-                          (tptr (Tstruct _lock_t noattr)))
-                        (Etempvar _l (tptr (Tstruct _lock_t noattr))))
-                      (Ssequence
-                        (Scall None
-                          (Evar _makelock (Tfunction
-                                            (Tcons (tptr tvoid) Tnil) tvoid
-                                            cc_default))
-                          ((Ecast
-                             (Etempvar _l (tptr (Tstruct _lock_t noattr)))
-                             (tptr tvoid)) :: nil))
-                        (Ssequence
-                          (Sset _t
-                            (Eaddrof
-                              (Ederef
-                                (Ebinop Oadd (Evar _tid (tarray tint 3))
-                                  (Etempvar _i tint) (tptr tint)) tint)
-                              (tptr tint)))
-                          (Scall None
-                            (Evar _spawn (Tfunction
-                                           (Tcons
-                                             (tptr (Tfunction
-                                                     (Tcons (tptr tvoid)
-                                                       Tnil) (tptr tvoid)
-                                                     cc_default))
-                                             (Tcons (tptr tvoid) Tnil)) tvoid
-                                           cc_default))
-                            ((Ecast
-                               (Eaddrof
-                                 (Evar _f (Tfunction
-                                            (Tcons (tptr tvoid) Tnil)
-                                            (tptr tvoid) cc_default))
-                                 (tptr (Tfunction (Tcons (tptr tvoid) Tnil)
-                                         (tptr tvoid) cc_default)))
-                               (tptr tvoid)) :: (Etempvar _t (tptr tvoid)) ::
-                             nil)))))))
-                (Sset _i
-                  (Ebinop Oadd (Etempvar _i tint)
-                    (Econst_int (Int.repr 1) tint) tint))))
+              (Scall (Some _t'1)
+                (Evar _q_new (Tfunction Tnil (tptr (Tstruct _queue_t noattr))
+                               cc_default)) nil)
+              (Sassign (Evar _q0 (tptr (Tstruct _queue_t noattr)))
+                (Etempvar _t'1 (tptr (Tstruct _queue_t noattr)))))
             (Ssequence
               (Ssequence
-                (Sset _i__1 (Econst_int (Int.repr 0) tint))
+                (Sset _i (Econst_int (Int.repr 0) tint))
                 (Sloop
                   (Ssequence
-                    (Sifthenelse (Ebinop Olt (Etempvar _i__1 tint)
-                                   (Econst_int (Int.repr 9) tint) tint)
+                    (Sifthenelse (Ebinop Olt (Etempvar _i tint)
+                                   (Econst_int (Int.repr 3) tint) tint)
                       Sskip
                       Sbreak)
                     (Ssequence
                       (Ssequence
-                        (Scall (Some _t'3)
+                        (Scall (Some _t'2)
                           (Evar _malloc (Tfunction (Tcons tuint Tnil)
                                           (tptr tvoid) cc_default))
-                          ((Esizeof tint tuint) :: nil))
-                        (Sset _d
-                          (Ecast (Etempvar _t'3 (tptr tvoid)) (tptr tint))))
+                          ((Esizeof (Tstruct _lock_t noattr) tuint) :: nil))
+                        (Sset _l
+                          (Ecast (Etempvar _t'2 (tptr tvoid))
+                            (tptr (Tstruct _lock_t noattr)))))
                       (Ssequence
-                        (Sassign (Ederef (Etempvar _d (tptr tint)) tint)
-                          (Etempvar _i__1 tint))
-                        (Scall None
-                          (Evar _q_add (Tfunction
-                                         (Tcons
-                                           (tptr (Tstruct _queue_t noattr))
-                                           (Tcons (tptr tvoid) Tnil)) tvoid
-                                         cc_default))
-                          ((Evar _q0 (tptr (Tstruct _queue_t noattr))) ::
-                           (Etempvar _d (tptr tint)) :: nil)))))
-                  (Sset _i__1
-                    (Ebinop Oadd (Etempvar _i__1 tint)
-                      (Econst_int (Int.repr 1) tint) tint))))
-              (Ssequence
-                (Ssequence
-                  (Sset _i__2 (Econst_int (Int.repr 0) tint))
-                  (Sloop
-                    (Ssequence
-                      (Sifthenelse (Ebinop Olt (Etempvar _i__2 tint)
-                                     (Econst_int (Int.repr 3) tint) tint)
-                        Sskip
-                        Sbreak)
-                      (Ssequence
-                        (Sset _l__1
+                        (Sassign
                           (Ederef
                             (Ebinop Oadd
                               (Evar _thread_locks (tarray (tptr (Tstruct _lock_t noattr)) 3))
-                              (Etempvar _i__2 tint)
+                              (Etempvar _i tint)
                               (tptr (tptr (Tstruct _lock_t noattr))))
-                            (tptr (Tstruct _lock_t noattr))))
+                            (tptr (Tstruct _lock_t noattr)))
+                          (Etempvar _l (tptr (Tstruct _lock_t noattr))))
                         (Ssequence
                           (Scall None
-                            (Evar _acquire (Tfunction
-                                             (Tcons (tptr tvoid) Tnil) tvoid
-                                             cc_default))
-                            ((Etempvar _l__1 (tptr (Tstruct _lock_t noattr))) ::
-                             nil))
+                            (Evar _makelock (Tfunction
+                                              (Tcons (tptr tvoid) Tnil) tvoid
+                                              cc_default))
+                            ((Ecast
+                               (Etempvar _l (tptr (Tstruct _lock_t noattr)))
+                               (tptr tvoid)) :: nil))
                           (Ssequence
+                            (Sset _t
+                              (Eaddrof
+                                (Ederef
+                                  (Ebinop Oadd (Evar _tid (tarray tint 3))
+                                    (Etempvar _i tint) (tptr tint)) tint)
+                                (tptr tint)))
                             (Scall None
-                              (Evar _freelock2 (Tfunction
-                                                 (Tcons (tptr tvoid) Tnil)
-                                                 tvoid cc_default))
-                              ((Etempvar _l__1 (tptr (Tstruct _lock_t noattr))) ::
-                               nil))
-                            (Scall None
-                              (Evar _free (Tfunction
-                                            (Tcons (tptr tvoid) Tnil) tvoid
-                                            cc_default))
-                              ((Etempvar _l__1 (tptr (Tstruct _lock_t noattr))) ::
-                               nil))))))
-                    (Sset _i__2
-                      (Ebinop Oadd (Etempvar _i__2 tint)
+                              (Evar _spawn (Tfunction
+                                             (Tcons
+                                               (tptr (Tfunction
+                                                       (Tcons (tptr tvoid)
+                                                         Tnil) (tptr tvoid)
+                                                       cc_default))
+                                               (Tcons (tptr tvoid) Tnil))
+                                             tvoid cc_default))
+                              ((Ecast
+                                 (Eaddrof
+                                   (Evar _f (Tfunction
+                                              (Tcons (tptr tvoid) Tnil)
+                                              (tptr tvoid) cc_default))
+                                   (tptr (Tfunction (Tcons (tptr tvoid) Tnil)
+                                           (tptr tvoid) cc_default)))
+                                 (tptr tvoid)) ::
+                               (Etempvar _t (tptr tvoid)) :: nil)))))))
+                  (Sset _i
+                    (Ebinop Oadd (Etempvar _i tint)
+                      (Econst_int (Int.repr 1) tint) tint))))
+              (Ssequence
+                (Ssequence
+                  (Sset _i__1 (Econst_int (Int.repr 0) tint))
+                  (Sloop
+                    (Ssequence
+                      (Sifthenelse (Ebinop Olt (Etempvar _i__1 tint)
+                                     (Econst_int (Int.repr 9) tint) tint)
+                        Sskip
+                        Sbreak)
+                      (Ssequence
+                        (Ssequence
+                          (Scall (Some _t'3)
+                            (Evar _malloc (Tfunction (Tcons tuint Tnil)
+                                            (tptr tvoid) cc_default))
+                            ((Esizeof tint tuint) :: nil))
+                          (Sset _d
+                            (Ecast (Etempvar _t'3 (tptr tvoid)) (tptr tint))))
+                        (Ssequence
+                          (Sassign (Ederef (Etempvar _d (tptr tint)) tint)
+                            (Etempvar _i__1 tint))
+                          (Scall None
+                            (Evar _q_add (Tfunction
+                                           (Tcons
+                                             (tptr (Tstruct _queue_t noattr))
+                                             (Tcons (tptr tvoid) Tnil)) tvoid
+                                           cc_default))
+                            ((Etempvar _q1 (tptr (Tstruct _queue_t noattr))) ::
+                             (Etempvar _d (tptr tint)) :: nil)))))
+                    (Sset _i__1
+                      (Ebinop Oadd (Etempvar _i__1 tint)
                         (Econst_int (Int.repr 1) tint) tint))))
                 (Ssequence
-                  (Sset _q1 (Evar _q0 (tptr (Tstruct _queue_t noattr))))
                   (Ssequence
-                    (Scall None
-                      (Evar _q_del (Tfunction
-                                     (Tcons (tptr (Tstruct _queue_t noattr))
-                                       Tnil) tvoid cc_default))
-                      ((Etempvar _q1 (tptr (Tstruct _queue_t noattr))) ::
-                       nil))
-                    (Ssequence
-                      (Sset _i__3 (Econst_int (Int.repr 0) tint))
-                      (Sloop
+                    (Sset _i__2 (Econst_int (Int.repr 0) tint))
+                    (Sloop
+                      (Ssequence
+                        (Sifthenelse (Ebinop Olt (Etempvar _i__2 tint)
+                                       (Econst_int (Int.repr 3) tint) tint)
+                          Sskip
+                          Sbreak)
                         (Ssequence
-                          (Sifthenelse (Ebinop Olt (Etempvar _i__3 tint)
-                                         (Econst_int (Int.repr 3) tint) tint)
-                            Sskip
-                            Sbreak)
+                          (Sset _l__1
+                            (Ederef
+                              (Ebinop Oadd
+                                (Evar _thread_locks (tarray (tptr (Tstruct _lock_t noattr)) 3))
+                                (Etempvar _i__2 tint)
+                                (tptr (tptr (Tstruct _lock_t noattr))))
+                              (tptr (Tstruct _lock_t noattr))))
                           (Ssequence
-                            (Sset _j (Econst_int (Int.repr 0) tint))
-                            (Sloop
-                              (Ssequence
-                                (Sifthenelse (Ebinop Olt (Etempvar _j tint)
-                                               (Econst_int (Int.repr 3) tint)
-                                               tint)
-                                  Sskip
-                                  Sbreak)
-                                (Scall None
-                                  (Evar _printf (Tfunction
-                                                  (Tcons (tptr tschar) Tnil)
-                                                  tint
-                                                  {|cc_vararg:=true; cc_unproto:=false; cc_structret:=false|}))
-                                  ((Evar ___stringlit_1 (tarray tschar 4)) ::
-                                   (Ederef
-                                     (Ebinop Oadd
-                                       (Ederef
-                                         (Ebinop Oadd
-                                           (Evar _results (tarray (tarray tint 3) 3))
-                                           (Etempvar _i__3 tint)
-                                           (tptr (tarray tint 3)))
-                                         (tarray tint 3)) (Etempvar _j tint)
-                                       (tptr tint)) tint) :: nil)))
-                              (Sset _j
-                                (Ebinop Oadd (Etempvar _j tint)
-                                  (Econst_int (Int.repr 1) tint) tint)))))
-                        (Sset _i__3
-                          (Ebinop Oadd (Etempvar _i__3 tint)
-                            (Econst_int (Int.repr 1) tint) tint)))))))))))))
+                            (Scall None
+                              (Evar _acquire (Tfunction
+                                               (Tcons (tptr tvoid) Tnil)
+                                               tvoid cc_default))
+                              ((Etempvar _l__1 (tptr (Tstruct _lock_t noattr))) ::
+                               nil))
+                            (Ssequence
+                              (Scall None
+                                (Evar _freelock2 (Tfunction
+                                                   (Tcons (tptr tvoid) Tnil)
+                                                   tvoid cc_default))
+                                ((Etempvar _l__1 (tptr (Tstruct _lock_t noattr))) ::
+                                 nil))
+                              (Scall None
+                                (Evar _free (Tfunction
+                                              (Tcons (tptr tvoid) Tnil) tvoid
+                                              cc_default))
+                                ((Etempvar _l__1 (tptr (Tstruct _lock_t noattr))) ::
+                                 nil))))))
+                      (Sset _i__2
+                        (Ebinop Oadd (Etempvar _i__2 tint)
+                          (Econst_int (Int.repr 1) tint) tint))))
+                  (Scall None
+                    (Evar _q_del (Tfunction
+                                   (Tcons (tptr (Tstruct _queue_t noattr))
+                                     Tnil) tvoid cc_default))
+                    ((Etempvar _q1 (tptr (Tstruct _queue_t noattr))) :: nil))))))))))
   (Sreturn (Some (Econst_int (Int.repr 0) tint))))
 |}.
 
@@ -975,8 +932,7 @@ Definition composites : list composite_definition :=
 
 Definition prog : Clight.program := {|
 prog_defs :=
-((___stringlit_1, Gvar v___stringlit_1) ::
- (___builtin_fabs,
+((___builtin_fabs,
    Gfun(External (EF_builtin "__builtin_fabs"
                    (mksignature (AST.Tfloat :: nil) (Some AST.Tfloat)
                      cc_default)) (Tcons tdouble Tnil) tdouble cc_default)) ::
@@ -1203,12 +1159,6 @@ prog_defs :=
                      {|cc_vararg:=true; cc_unproto:=false; cc_structret:=false|}))
      (Tcons tint Tnil) tvoid
      {|cc_vararg:=true; cc_unproto:=false; cc_structret:=false|})) ::
- (_printf,
-   Gfun(External (EF_external "printf"
-                   (mksignature (AST.Tint :: nil) (Some AST.Tint)
-                     {|cc_vararg:=true; cc_unproto:=false; cc_structret:=false|}))
-     (Tcons (tptr tschar) Tnil) tint
-     {|cc_vararg:=true; cc_unproto:=false; cc_structret:=false|})) ::
  (_exit,
    Gfun(External (EF_external "exit"
                    (mksignature (AST.Tint :: nil) None cc_default))
@@ -1276,7 +1226,7 @@ prog_public :=
  _q_tryremove :: _q_add :: _q_del :: _q_new :: _surely_malloc ::
  _signalcond :: _waitcond :: _freecond :: _makecond :: _spawn :: _release2 ::
  _freelock2 :: _release :: _acquire :: _freelock :: _makelock :: _malloc ::
- _free :: _exit :: _printf :: ___builtin_debug :: ___builtin_nop ::
+ _free :: _exit :: ___builtin_debug :: ___builtin_nop ::
  ___builtin_write32_reversed :: ___builtin_write16_reversed ::
  ___builtin_read32_reversed :: ___builtin_read16_reversed ::
  ___builtin_fnmsub :: ___builtin_fnmadd :: ___builtin_fmsub ::
